De la siguiente funci√≥n de recurrencia, demostrar sus valores previos:

$f(n)=f(n-1)+1$

Donde el caso base es: $f(1)=0$ y con $n=5$.

$Solucion:$

con $n=5$ :
- $f(5)=f(5-1)+1$
- $f(5)=f(4)+1$
- donde $f(5)=f(4)+1$ .
con $n=4$ :
- $f(4)=f(4-1)+1$
- $f(4)=f(3)+1$
con $n=3$ :
- $f(3)=f(3-1)+1$
- $f(3)=f(2)+1$
con $n=2$ :
- $f(2)=f(2-1)+1$
- $f(2)=f(1)+1$
Pero como $f(1)=0$ $entonces$: $f(2)=0+1$ donde $f(2)= 1$:
- $f(2)=0+1=1$
- $f(3)=f(2)+1=1+1=2$
- $f(4)=f(3)+1=2+1=3$
- $f(5)=f(4)+1=3+1=4$
- 

